tests/lean/Hashmap/Properties.lean
@@ -67,12 +67,30 @@ theorem hash_mod_key_eq : hash_mod_key k l = k.val % l := by
 def slot_s_inv_hash (l i : Int) (ls : List (Usize × α)) : Prop :=
   ls.allP (λ (k, _) => hash_mod_key k l = i)
 
-@[simp]
 def slot_s_inv (l i : Int) (ls : List (Usize × α)) : Prop :=
   distinct_keys ls ∧
   slot_s_inv_hash l i ls
 
 def slot_t_inv (l i : Int) (s : AList α) : Prop := slot_s_inv l i s.v
+
+@[simp] theorem distinct_keys_nil : @distinct_keys α [] := by simp [distinct_keys]
+@[simp] theorem slot_s_inv_hash_nil : @slot_s_inv_hash l i α [] := by simp [slot_s_inv_hash]
+@[simp] theorem slot_s_inv_nil : @slot_s_inv α l i [] := by simp [slot_s_inv]
+@[simp] theorem slot_t_inv_nil : @slot_t_inv α l i .Nil := by simp [slot_t_inv]
+
+@[simp] theorem distinct_keys_cons (kv : Usize × α) (tl : List (Usize × α)) :
+  distinct_keys (kv :: tl) ↔ ((tl.allP fun (k', _) => ¬↑kv.1 = ↑k') ∧ distinct_keys tl) := by simp [distinct_keys]
+
+@[simp] theorem slot_s_inv_hash_cons (kv : Usize × α) (tl : List (Usize × α)) :
+  slot_s_inv_hash l i (kv :: tl) ↔
+    (hash_mod_key kv.1 l = i ∧ tl.allP (λ (k, _) => hash_mod_key k l = i) ∧ slot_s_inv_hash l i tl) :=
+  by simp [slot_s_inv_hash]
+
+@[simp] theorem slot_s_inv_cons (kv : Usize × α) (tl : List (Usize × α)) :
+  slot_s_inv l i (kv :: tl) ↔
+    ((tl.allP fun (k', _) => ¬↑kv.1 = ↑k') ∧ distinct_keys tl ∧
+     hash_mod_key kv.1 l = i ∧ tl.allP (λ (k, _) => hash_mod_key k l = i) ∧ slot_s_inv l i tl) := by
+    simp [slot_s_inv]; tauto
 
 -- Interpret the hashmap as a list of lists
 def v (hm : HashMap α) : List (List (Usize × α)) :=
@@ -94,19 +112,58 @@ def slots_t_inv (s : alloc.vec.Vec (AList α)) : Prop :=
   slots_s_inv s.v
 
 @[simp]
-def base_inv (hm : HashMap α) : Prop :=
+def slots_s_lookup (s : List (AList α)) (k : Usize) : Option α :=
+  let i := hash_mod_key k s.len
+  let slot := s.index i
+  slot.lookup k
+
+abbrev Slots α := alloc.vec.Vec (AList α)
+
+abbrev Slots.lookup (s : Slots α) (k : Usize) := slots_s_lookup s.val k
+
+abbrev Slots.al_v (s : Slots α) := (s.val.map AList.v).flatten
+
+def lookup (hm : HashMap α) (k : Usize) : Option α :=
+  slots_s_lookup hm.slots.val k
+
+@[simp]
+abbrev len_s (hm : HashMap α) : Int := hm.al_v.len
+
+instance : Membership Usize (HashMap α) where
+  mem k hm := hm.lookup k ≠ none
+
+/- Activate the ↑ notation -/
+attribute [coe] HashMap.v
+
+abbrev inv_load (hm : HashMap α) : Prop :=
+  let capacity := hm.slots.val.len
+  -- TODO: let (dividend, divisor) := hm.max_load_factor introduces field notation .2, etc.
+  let dividend := hm.max_load_factor.1
+  let divisor := hm.max_load_factor.2
+  0 < dividend.val ∧ dividend < divisor ∧
+  capacity * dividend >= divisor ∧
+  hm.max_load = (capacity * dividend) / divisor
+
+@[simp]
+def inv_base (hm : HashMap α) : Prop :=
   -- [num_entries] correctly tracks the number of entries
   hm.num_entries.val = hm.al_v.len ∧
   -- Slots invariant
   slots_t_inv hm.slots ∧
   -- The capacity must be > 0 (otherwise we can't resize)
-  0 < hm.slots.length
-  -- TODO: load computation
+  0 < hm.slots.length ∧ -- TODO: normalization lemmas for comparison
+  -- Load computation
+  inv_load hm
 
 def inv (hm : HashMap α) : Prop :=
   -- Base invariant
-  base_inv hm
+  inv_base hm
   -- TODO: either the hashmap is not overloaded, or we can't resize it
+
+def frame_load (hm nhm : HashMap α) : Prop :=
+  nhm.max_load_factor = hm.max_load_factor ∧
+  nhm.max_load = hm.max_load ∧
+  nhm.saturated = hm.saturated
 
 -- This rewriting lemma is problematic below
 attribute [-simp] Bool.exists_bool
@@ -114,6 +171,116 @@ attribute [-simp] Bool.exists_bool
 -- The proof below is a bit expensive, so we need to increase the maximum number
 -- of heart beats
 set_option maxHeartbeats 1000000
+open AList
+
+@[pspec]
+theorem allocate_slots_spec {α : Type} (slots : alloc.vec.Vec (AList α)) (n : Usize)
+  (Hslots : ∀ (i : Int), 0 ≤ i → i < slots.len → slots.val.index i = Nil)
+  (Hlen : slots.len + n.val ≤ Usize.max) :
+  ∃ slots1, allocate_slots α slots n = ok slots1 ∧
+  (∀ (i : Int), 0 ≤ i → i < slots1.len → slots1.val.index i = Nil) ∧
+  slots1.len = slots.len + n.val := by
+  rw [allocate_slots]
+  rw [allocate_slots_loop]
+  if h: 0 < n.val then
+    simp [h]
+    -- TODO: progress fails here (maximum recursion depth reached)
+    -- progress as ⟨ slots1 .. ⟩
+    have ⟨ slots1, hEq, _ ⟩ := alloc.vec.Vec.push_spec slots Nil (by scalar_tac)
+    simp [hEq]; clear hEq
+    progress as ⟨ n1 ⟩
+    have Hslots1Nil :
+      ∀ (i : ℤ), 0 ≤ i → i < ↑(alloc.vec.Vec.len (AList α) slots1) → slots1.val.index i = Nil := by
+      intro i h0 h1
+      simp [*]
+      if hi : i < slots.val.len then
+        simp [*]
+      else
+        simp_all
+        have : i - slots.val.len = 0 := by scalar_tac
+        simp [*]
+    have Hslots1Len : alloc.vec.Vec.len (AList α) slots1 + n1.val ≤ Usize.max := by
+      simp_all
+    -- TODO: progress fails here (maximum recursion depth reached)
+    -- This probably comes from the fact that allocate_slots is reducible and applied an infinite number
+    -- of times
+    -- progress as ⟨ slots2 .. ⟩
+    -- TODO: bug here as well
+    stop
+    have ⟨ slots2, hEq, _, _ ⟩ := allocate_slots_spec slots1 n1 (by assumption) (by assumption)
+    stop
+    rw [allocate_slots] at hEq; rw [hEq]; clear hEq
+    simp
+    constructor
+    . intro i h0 h1
+      simp_all
+    . simp_all
+  else
+    simp [h]
+    simp_all
+    scalar_tac
+
+theorem forall_nil_imp_flatten_len_zero (slots : List (List α))
+  (Hnil : ∀ i, 0 ≤ i → i < slots.len → slots.index i = []) :
+  slots.flatten = [] := by
+  induction slots <;> simp_all
+  have Hhead := Hnil 0 (by simp) (by scalar_tac)
+  simp_all; clear Hhead
+  rename _ → _ => Hind
+  apply Hind
+  intros i h0 h1
+  have := Hnil (i + 1) (by scalar_tac) (by scalar_tac)
+  have : 0 < i + 1 := by scalar_tac
+  simp_all
+
+@[pspec]
+theorem new_with_capacity_spec
+  (capacity : Usize) (max_load_dividend : Usize) (max_load_divisor : Usize)
+  (Hcapa : 0 < capacity.val)
+  (Hfactor : 0 < max_load_dividend.val ∧ max_load_dividend.val < max_load_divisor.val ∧
+             capacity.val * max_load_dividend.val ≤ Usize.max ∧
+             capacity.val * max_load_dividend.val ≥ max_load_divisor)
+  (Hdivid : 0 < max_load_divisor.val) :
+  ∃ hm, new_with_capacity α capacity max_load_dividend max_load_divisor = ok hm ∧
+  hm.inv ∧ hm.len_s = 0 ∧ ∀ k, hm.lookup k = none := by
+  rw [new_with_capacity]
+  progress as ⟨ slots, Hnil .. ⟩
+  . intros; simp [alloc.vec.Vec.new] at *; scalar_tac
+  . simp [alloc.vec.Vec.new]; scalar_tac
+  . progress as ⟨ i1 .. ⟩
+    progress as ⟨ i2 .. ⟩
+    simp [inv, inv_load]
+    have : (Slots.al_v slots).len = 0 := by
+      have := forall_nil_imp_flatten_len_zero (slots.val.map AList.v)
+        (by intro i h0 h1; simp_all)
+      simp_all
+    have : 0 < slots.val.len := by simp_all [alloc.vec.Vec.len, alloc.vec.Vec.new]
+    have : slots_t_inv slots := by
+      simp [slots_t_inv, slot_t_inv]
+      intro i h0 h1
+      simp_all
+    split_conjs
+    . simp_all [al_v, Slots.al_v, v]
+    . assumption
+    . scalar_tac
+    . simp_all [alloc.vec.Vec.len, alloc.vec.Vec.new]
+    . simp_all
+    . simp_all [alloc.vec.Vec.len, alloc.vec.Vec.new]
+    . simp_all [alloc.vec.Vec.len, alloc.vec.Vec.new]
+    . simp_all [al_v, Slots.al_v, v]
+    . simp [lookup]
+      intro k
+      have : 0 ≤ k.val % slots.val.len := by apply Int.emod_nonneg; scalar_tac
+      have : k.val % slots.val.len < slots.val.len := by apply Int.emod_lt_of_pos; scalar_tac
+      simp [*]
+
+@[pspec]
+theorem new_spec (α : Type) :
+  ∃ hm, new α = ok hm ∧
+  hm.inv ∧ hm.len_s = 0 ∧ ∀ k, hm.lookup k = none := by
+  rw [new]
+  progress as ⟨ hm ⟩
+  simp_all
 
 theorem insert_in_list_spec_aux {α : Type} (l : Int) (key: Usize) (value: α) (l0: AList α)
   (hinv : slot_s_inv_hash l (hash_mod_key key l) l0.v)
@@ -141,21 +308,19 @@ theorem insert_in_list_spec_aux {α : Type} (l : Int) (key: Usize) (value: α) (
     exists true -- TODO: why do we need to do this?
     simp [insert_in_list]
     rw [insert_in_list_loop]
-    simp (config := {contextual := true})
-      [AList.v, slot_s_inv_hash, distinct_keys, List.pairwise_rel]
+    simp (config := {contextual := true}) [AList.v]
   | Cons k v tl0 =>
      if h: k = key then
        rw [insert_in_list]
        rw [insert_in_list_loop]
        simp [h]
-       exists false; simp -- TODO: why do we need to do this?
+       exists false; simp only [true_and, exists_eq_left', List.lookup', ↓reduceIte, AList.v_cons] -- TODO: why do we need to do this?
        split_conjs
        . intros; simp [*]
-       . simp [AList.v, slot_s_inv_hash] at *
-         simp [*]
-       . simp [*, distinct_keys] at *
-         apply hdk
-       . tauto
+       . simp_all [slot_s_inv_hash]
+       . simp at hinv; tauto
+       . simp_all [slot_s_inv_hash]
+       . simp_all
      else
        rw [insert_in_list]
        rw [insert_in_list_loop]
@@ -199,18 +364,6 @@ theorem insert_in_list_spec {α : Type} (l : Int) (key: Usize) (value: α) (l0: 
   exists b
   exists l1
 
-@[simp]
-def slots_t_lookup (s : List (AList α)) (k : Usize) : Option α :=
-  let i := hash_mod_key k s.len
-  let slot := s.index i
-  slot.lookup k
-
-def lookup (hm : HashMap α) (k : Usize) : Option α :=
-  slots_t_lookup hm.slots.val k
-
-@[simp]
-abbrev len_s (hm : HashMap α) : Int := hm.al_v.len
-
 -- Remark: α and β must live in the same universe, otherwise the
 -- bind doesn't work
 theorem if_update_eq
@@ -235,6 +388,7 @@ set_option pp.coercions false -- do not print coercions with ↑ (this doesn't p
 -- of heart beats
 set_option maxHeartbeats 2000000
 
+@[pspec]
 theorem insert_no_resize_spec {α : Type} (hm : HashMap α) (key : Usize) (value : α)
   (hinv : hm.inv) (hnsat : hm.lookup key = none → hm.len_s < Usize.max) :
   ∃ nhm, hm.insert_no_resize α key value = ok nhm  ∧
@@ -271,7 +425,7 @@ theorem insert_no_resize_spec {α : Type} (hm : HashMap α) (key : Usize) (value
     simp [slot_t_inv, hhm] at h
     simp [h, hhm, h_leq]
   have hd : distinct_keys l.v := by
-    simp [inv, slots_t_inv, slot_t_inv] at hinv
+    simp [inv, slots_t_inv, slot_t_inv, slot_s_inv] at hinv
     have h := hinv.right.left hash_mod.val (by assumption) (by assumption)
     simp [h, h_leq]
   progress as ⟨ inserted, l0, _, _, _, _, hlen .. ⟩
@@ -300,7 +454,12 @@ theorem insert_no_resize_spec {α : Type} (hm : HashMap α) (key : Usize) (value
   -- TODO: update progress to automate that
   -- TODO: later I don't want to inline nhm - we need to control simp: deactivate
   -- zeta reduction? For now I have to do this peculiar manipulation
-  have ⟨ nhm, nhm_eq ⟩ := @mk_opaque (HashMap α) { num_entries := i0, max_load_factor := hm.max_load_factor, max_load := hm.max_load, slots := v }
+  have ⟨ nhm, nhm_eq ⟩ := @mk_opaque (HashMap α) {
+      num_entries := i0,
+      max_load_factor := hm.max_load_factor,
+      max_load := hm.max_load,
+      saturated := hm.saturated,
+      slots := v }
   exists nhm
   have hupdt : lookup nhm key = some value := by
     simp [lookup, List.lookup] at *
@@ -338,14 +497,12 @@ theorem insert_no_resize_spec {α : Type} (hm : HashMap α) (key : Usize) (value
     match hm.lookup key with
     | none => nhm.len_s = hm.len_s + 1
     | some _ => nhm.len_s = hm.len_s := by
-    simp only [lookup, List.lookup, len_s, al_v, HashMap.v, slots_t_lookup] at *
+    simp only [lookup, List.lookup, len_s, al_v, HashMap.v, slots_s_lookup] at *
     -- We have to do a case disjunction
-    simp_all
-    simp [List.update_map_eq]
+    simp_all [List.map_update_eq]
     -- TODO: dependent rewrites
     have _ : key.val % hm.slots.val.len < (List.map AList.v hm.slots.val).len := by
       simp [*]
-    simp [List.len_flatten_update_eq, *]
     split <;>
     rename_i heq <;>
     simp [heq] at hlen <;>
@@ -366,20 +523,733 @@ theorem insert_no_resize_spec {α : Type} (hm : HashMap α) (key : Usize) (value
     . simp [slots_t_inv, slot_t_inv] at *
       intro i hipos _
       have _ := hinv.right.left i hipos (by simp_all)
-      simp [hhm, h_veq, nhm_eq] at * -- TODO: annoying, we do that because simp_all fails below
       -- We need a case disjunction
-      if h_ieq : i = key.val % List.len hm.slots.val then
-        -- TODO: simp_all fails: "(deterministic) timeout at 'whnf'"
-        -- Also, it is annoying to do this kind
-        -- of rewritings by hand. We could have a different simp
-        -- which safely substitutes variables when we have an
-        -- equality `x = ...` and `x` doesn't appear in the rhs
-        simp [h_ieq] at *
-        simp [*]
-      else
-        simp [*]
+      cases h_ieq : i == key.val % List.len hm.slots.val <;> simp_all [slot_s_inv]
     . simp [hinv, h_veq, nhm_eq]
+    . simp_all [frame_load, inv_base, inv_load]
   simp_all
+
+theorem slot_allP_not_key_lookup (slot : AList T) (h : slot.v.allP fun (k', _) => ¬k = k') :
+  slot.lookup k = none := by
+  induction slot <;> simp_all
+
+@[pspec]
+theorem move_elements_from_list_spec
+  {T : Type} (ntable : HashMap T) (slot : AList T)
+  (hinv : ntable.inv)
+  {l i : Int} (hSlotInv : slot_t_inv l i slot)
+  (hDisjoint1 : ∀ key v, ntable.lookup key = some v → slot.lookup key = none)
+  (hDisjoint2 : ∀ key v, slot.lookup key = some v → ntable.lookup key = none)
+  (hLen : ntable.al_v.len + slot.v.len ≤ Usize.max)
+  :
+  ∃ ntable1, ntable.move_elements_from_list T slot = ok ntable1 ∧
+  ntable1.inv ∧
+  (∀ key v, ntable1.lookup key = some v → ntable.lookup key = some v ∨ slot.lookup key = some v) ∧
+  (∀ key v, ntable.lookup key = some v → ntable1.lookup key = some v) ∧
+  (∀ key v, slot.lookup key = some v → ntable1.lookup key = some v) ∧
+  ntable1.al_v.len = ntable.al_v.len + slot.v.len
+  := by
+  rw [move_elements_from_list]; rw [move_elements_from_list_loop]
+  cases slot with
+  | Nil =>
+    simp [hinv]
+  | Cons key value slot1 =>
+    simp
+    have hLookupKey : ntable.lookup key = none := by
+      by_contra
+      cases h: ntable.lookup key <;> simp_all
+      have h := hDisjoint1 _ _ h
+      simp_all
+    have : ntable.lookup key = none → ntable.len_s < Usize.max := by simp_all; scalar_tac
+    progress as ⟨ ntable1, _, hLookup11, hLookup12, hLength1 ⟩
+    simp [hLookupKey] at hLength1
+    have hTable1LookupImp : ∀ (key : Usize) (v : T), ntable1.lookup key = some v → slot1.lookup key = none := by
+      intro key' v hLookup
+      if h: key = key' then
+        simp_all [slot_t_inv]
+        apply slot_allP_not_key_lookup
+        simp_all
+      else
+        simp_all
+        cases h: ntable.lookup key' <;> simp_all
+        have := hDisjoint1 _ _ h
+        simp_all
+    have hSlot1LookupImp : ∀ (key : Usize) (v : T), slot1.lookup key = some v → ntable1.lookup key = none := by
+      intro key' v hLookup
+      if h: key' = key then
+        by_contra
+        rename _ => hNtable1NotNone
+        cases h: ntable1.lookup key' <;> simp [h] at hNtable1NotNone
+        have := hTable1LookupImp _ _ h
+        simp_all
+      else
+        have := hLookup12 key' h
+        have := hDisjoint2 key' v
+        simp_all
+    have : ntable1.al_v.len + slot1.v.len ≤ Usize.max := by simp_all; scalar_tac
+    have : slot_t_inv l i slot1 := by
+      simp [slot_t_inv] at hSlotInv
+      simp [slot_t_inv, hSlotInv]
+    -- TODO: progress leads to: slot_t_inv i i slot1
+    -- progress as ⟨ ntable2 ⟩
+
+    have  ⟨ ntable2, hEq, hInv2, hLookup21, hLookup22, hLookup23, hLen1 ⟩ :=
+      move_elements_from_list_spec ntable1 slot1 (by assumption) (by assumption)
+          hTable1LookupImp hSlot1LookupImp (by assumption)
+    simp [hEq]; clear hEq
+    -- The conclusion
+    -- TODO: use aesop here
+    split_conjs
+    . simp [*]
+    . intro key' v hLookup
+      have := hLookup21 key' v
+      if h: key = key' then
+        have := hLookup22 key' v
+        have := hLookup23 key' v
+        have := hDisjoint1 key' v
+        have := hDisjoint2 key' v
+        have := hTable1LookupImp key' v
+        have := hSlot1LookupImp key' v
+        simp_all [Slots.lookup]
+      else have := hLookup12 key'; simp_all
+    . intro key' v hLookup1
+      if h: key' = key then
+        simp_all
+      else
+        have := hLookup12 key' h
+        have := hLookup22 key' v
+        simp_all
+    . intro key' v hLookup1
+      if h: key' = key then
+        have := hLookup22 key' v
+        simp_all
+      else
+        have := hLookup23 key' v
+        simp_all
+    . scalar_tac
+
+theorem slots_forall_nil_imp_lookup_none (slots : Slots T) (hLen : slots.val.len ≠ 0)
+  (hEmpty : ∀ j, 0 ≤ j → j < slots.val.len → slots.val.index j = AList.Nil) :
+  ∀ key, slots.lookup key = none := by
+  intro key
+  simp [Slots.lookup]
+  have : 0 ≤ key.val % slots.val.len := by
+    exact Int.emod_nonneg key.val hLen -- TODO: automate that
+  have : key.val % slots.val.len < slots.val.len := by
+    apply Int.emod_lt_of_pos
+    scalar_tac
+  have := hEmpty (key.val % slots.val.len) (by assumption) (by assumption)
+  simp [*]
+
+theorem slots_index_len_le_flatten_len (slots : List (AList α)) (i : Int) (h : 0 ≤ i ∧ i < slots.len) :
+  (slots.index i).len ≤ (List.map AList.v slots).flatten.len := by
+  match slots with
+  | [] =>
+    simp at *; scalar_tac
+  | slot :: slots' =>
+    simp at *
+    if hi : i = 0 then
+      simp_all; scalar_tac
+    else
+      have := slots_index_len_le_flatten_len slots' (i - 1) (by scalar_tac)
+      simp [*]
+      scalar_tac
+
+/- If we successfully lookup a key from a slot, the hash of the key modulo the number of slots must
+   be equal to the slot index.
+   TODO: remove?
+ -/
+theorem slots_inv_lookup_imp_eq (slots : Slots α) (hInv : slots_t_inv slots)
+  (i : Int) (hi : 0 ≤ i ∧ i < slots.val.len) (key : Usize) :
+  (slots.val.index i).lookup key ≠ none → i = key.val % slots.val.len := by
+  suffices hSlot : ∀ (slot : List (Usize × α)),
+           slot_s_inv slots.val.len i slot →
+           slot.lookup' key ≠ none →
+           i = key.val % slots.val.len
+  from by
+    rw [slots_t_inv, slots_s_inv] at hInv
+    replace hInv := hInv i hi.left hi.right
+    simp [slot_t_inv] at hInv
+    exact hSlot _ hInv
+  intro slot
+  induction slot <;> simp_all
+  intros; simp_all
+  split at * <;> simp_all
+
+-- TODO: remove?
+theorem slots_update_lookup_equiv (slots : Slots α) (hInv : slots_t_inv slots)
+  (i : Int) (hi : 0 ≤ i ∧ i < slots.val.len) (key : Usize) :
+  let slot := slots.val.index i
+  slot.lookup key ≠ none ∨ slots_s_lookup (slots.val.update i .Nil) key ≠ none ↔
+  slots.lookup key ≠ none := by
+  -- We need the following lemma to derive a contradiction
+  have := slots_inv_lookup_imp_eq slots hInv i hi key
+  cases hi : (key.val % slots.val.len) == i <;>
+  simp_all [Slots.lookup]
+
+/-theorem slots_update_lookup_imp
+  (slots slots1 : Slots α) (slot : AList α) (hInv : slots_t_inv slots) (i : Int) (hi : 0 ≤ i ∧ i < slots.val.len)
+  (hSlotsEq : slots.val = slots.val.update i slot) :
+  ∀ key v, slots1.lookup key = some v → slots.lookup key = some v ∨ slot.lookup key = some v-/
+
+theorem move_slots_updated_table_lookup_imp
+  (ntable ntable1 ntable2 : HashMap α) (slots slots1 : Slots α) (slot : AList α)
+  (hi : 0 ≤ i ∧ i < slots.val.len)
+  (hSlotsInv : slots_t_inv slots)
+  (hSlotEq : slot = slots.val.index i)
+  (hSlotsEq : slots1.val = slots.val.update i .Nil)
+  (hTableLookup : ∀ (key : Usize) (v : α), ntable1.lookup key = some v →
+                    ntable.lookup key = some v ∨ slot.lookup key = some v)
+  (hTable1Lookup : ∀ (key : Usize) (v : α), ntable2.lookup key = some v →
+                    ntable1.lookup key = some v ∨ Slots.lookup slots1 key = some v)
+  :
+  ∀ key v, ntable2.lookup key = some v → ntable.lookup key = some v ∨ slots.lookup key = some v := by
+  intro key v hLookup
+  replace hTableLookup := hTableLookup key v
+  replace hTable1Lookup := hTable1Lookup key v hLookup
+  cases hTable1Lookup with
+  | inl hTable1Lookup =>
+    replace hTableLookup := hTableLookup hTable1Lookup
+    cases hTableLookup <;> try simp [*]
+    right
+    have := slots_inv_lookup_imp_eq slots hSlotsInv i hi key (by simp_all)
+    simp_all [Slots.lookup]
+  | inr hTable1Lookup =>
+    right
+    -- The key can't be for the slot we replaced
+    if heq : key.val % slots.val.len = i then
+      simp_all [Slots.lookup]
+    else
+      simp_all [Slots.lookup]
+
+theorem move_one_slot_lookup_equiv {α : Type} (ntable ntable1 ntable2 : HashMap α)
+  (slot : AList α)
+  (slots slots1 : Slots α)
+  (i : Int) (h1 : i < slots.len)
+  (hSlotEq : slot = slots.val.index i)
+  (hSlots1Eq : slots1.val = slots.val.update i .Nil)
+  (hLookup1 : ∀ (key : Usize) (v : α), ntable.lookup key = some v → ntable1.lookup key = some v)
+  (hLookup2 : ∀ (key : Usize) (v : α), slot.lookup key = some v → ntable1.lookup key = some v)
+  (hLookup3 : ∀ (key : Usize) (v : α), ntable1.lookup key = some v → ntable2.lookup key = some v)
+  (hLookup4 : ∀ (key : Usize) (v : α), slots1.lookup key = some v → ntable2.lookup key = some v) :
+  (∀ key v, slots.lookup key = some v → ntable2.lookup key = some v) ∧
+  (∀ key v, ntable.lookup key = some v → ntable2.lookup key = some v) := by
+  constructor <;> intro key v hLookup
+  . if hi: key.val % slots.val.len = i then
+      -- We lookup in slot
+      have := hLookup2 key v
+      simp_all [Slots.lookup]
+      have := hLookup3 key v
+      simp_all
+    else
+      -- We lookup in slots
+      have := hLookup4 key v
+      simp_all [Slots.lookup]
+  . have := hLookup1 key v
+    have := hLookup3 key v
+    simp_all
+
+theorem slots_lookup_none_imp_slot_lookup_none
+  (slots : Slots α) (hInv : slots_t_inv slots) (i : Int) (hi : 0 ≤ i ∧ i < slots.val.len) :
+  ∀ (key : Usize), slots.lookup key = none → (slots.val.index i).lookup key = none := by
+  intro key hLookup
+  if heq : i = key.val % slots.val.len then
+    simp_all [Slots.lookup]
+  else
+    have := slots_inv_lookup_imp_eq slots hInv i (by scalar_tac) key
+    by_contra
+    simp_all
+
+theorem slot_lookup_not_none_imp_slots_lookup_not_none
+  (slots : Slots α) (hInv : slots_t_inv slots) (i : Int) (hi : 0 ≤ i ∧ i < slots.val.len) :
+  ∀ (key : Usize), (slots.val.index i).lookup key ≠ none → slots.lookup key ≠ none := by
+  intro key hLookup hNone
+  have := slots_lookup_none_imp_slot_lookup_none slots hInv i hi key hNone
+  apply hLookup this
+
+theorem slots_forall_nil_imp_al_v_nil (slots : Slots α)
+  (hEmpty : ∀ i, 0 ≤ i → i < slots.val.len → slots.val.index i = AList.Nil) :
+  slots.al_v = [] := by
+  suffices h :
+    ∀ (slots : List (AList α)),
+      (∀ (i : ℤ), 0 ≤ i → i < slots.len → slots.index i = Nil) →
+      (slots.map AList.v).flatten = [] from by
+      replace h := h slots.val (by intro i h0 h1; exact hEmpty i h0 h1)
+      simp_all
+  clear slots hEmpty
+  intro slots hEmpty
+  induction slots <;> simp_all
+  have hHead := hEmpty 0 (by simp) (by scalar_tac)
+  simp at hHead
+  simp [hHead]
+  rename (_ → _) => ih
+  apply ih; intro i h0 h1
+  replace hEmpty := hEmpty (i + 1) (by omega) (by omega)
+  -- TODO: simp at hEmpty
+  have : 0 < i + 1 := by omega
+  simp_all
+
+theorem move_elements_loop_spec
+  (n : Nat) -- We need this, otherwise we can't prove termination (the termination_by clauses can be expensive)
+  {α : Type} (ntable : HashMap α) (slots : Slots α)
+  (i : Usize)
+  (hn : n = slots.val.len - i.val) -- Condition for termination
+  (hi : i ≤ alloc.vec.Vec.len (AList α) slots)
+  (hinv : ntable.inv)
+  (hSlotsNonZero : slots.val.len ≠ 0)
+  (hSlotsInv : slots_t_inv slots)
+  (hEmpty : ∀ j, 0 ≤ j → j < i.val → slots.val.index j = AList.Nil)
+  (hDisjoint1 : ∀ key v, ntable.lookup key = some v → slots.lookup key = none)
+  (hDisjoint2 : ∀ key v, slots.lookup key = some v → ntable.lookup key = none)
+  (hLen : ntable.al_v.len + slots.al_v.len ≤ Usize.max)
+  :
+  ∃ ntable1 slots1, ntable.move_elements_loop α slots i = ok (ntable1, slots1) ∧
+  ntable1.inv ∧
+  ntable1.al_v.len = ntable.al_v.len + slots.al_v.len ∧
+  (∀ key v, ntable1.lookup key = some v → ntable.lookup key = some v ∨ slots.lookup key = some v) ∧
+  (∀ key v, slots.lookup key = some v → ntable1.lookup key = some v) ∧
+  (∀ key v, ntable.lookup key = some v → ntable1.lookup key = some v) ∧
+  (∀ (j : Int), 0 ≤ j → j < slots1.len → slots1.val.index j = AList.Nil)
+  := by
+  rw [move_elements_loop]
+  simp
+  if hi: i.val < slots.val.len then
+    -- Proof of termination: eliminate the case: n = 0
+    cases n; scalar_tac
+    rename ℕ => n
+    -- Continue the proof
+    have hIneq : 0 ≤ i.val ∧ i.val < slots.val.len := by scalar_tac
+    simp [hi]
+    progress as ⟨ slot, index_back, hSlotEq, hIndexBack ⟩
+    rw [hIndexBack]; clear hIndexBack
+    have hInvSlot : slot_t_inv slots.val.len i.val slot := by
+      simp [slots_t_inv] at hSlotsInv
+      simp [*]
+    have ntableLookupImpSlot :
+      ∀ (key : Usize) (v : α), ntable.lookup key = some v → slot.lookup key = none := by
+      intro key v hLookup
+      by_contra
+      have : i.val = key.val % slots.val.len := by
+        apply slots_inv_lookup_imp_eq slots hSlotsInv i.val (by scalar_tac)
+        simp_all
+      cases h: slot.lookup key <;> simp_all
+      have := hDisjoint2 _ _ h
+      simp_all
+    have slotLookupImpNtable :
+      ∀ (key : Usize) (v : α), slot.lookup key = some v → ntable.lookup key = none := by
+      intro key v hLookup
+      by_contra
+      cases h : ntable.lookup key <;> simp_all
+      have := ntableLookupImpSlot _ _ h
+      simp_all
+
+    have : ntable.al_v.len + slot.v.len ≤ Usize.max := by
+      have := slots_index_len_le_flatten_len slots.val i.val (by scalar_tac)
+      simp_all [Slots.al_v]; scalar_tac
+    progress as ⟨ ntable1, _, hDisjointNtable1, hLookup11, hLookup12, hLen1 ⟩ -- TODO: decompose post-condition by default
+    progress as ⟨ i' .. ⟩
+    progress as ⟨ slots1, hSlots1Eq .. ⟩
+    have : i' ≤ alloc.vec.Vec.len (AList α) slots1 := by simp_all [alloc.vec.Vec.len]; scalar_tac
+    have : slots_t_inv slots1 := by
+      simp [slots_t_inv] at *
+      intro j h0 h1
+      cases h: j == i.val <;> simp_all
+
+    have ntable1LookupImpSlots1 : ∀ (key : Usize) (v : α), ntable1.lookup key = some v → Slots.lookup slots1 key = none := by
+      intro key v hLookup
+      cases hDisjointNtable1 _ _ hLookup with
+      | inl h =>
+        have := ntableLookupImpSlot _ _ h
+        have := hDisjoint1 _ _ h
+        cases heq : i == key.val % slots.val.len <;> simp_all [Slots.lookup]
+      | inr h =>
+        --have h1 := hLookup12 _ _ h
+        have heq : i = key.val % slots.val.len := by
+          exact slots_inv_lookup_imp_eq slots hSlotsInv i.val hIneq key (by simp_all [Slots.lookup])
+        simp_all [Slots.lookup]
+
+    have : ∀ (key : Usize) (v : α), Slots.lookup slots1 key = some v → ntable1.lookup key = none := by
+      intro key v hLookup
+      by_contra h
+      cases h : ntable1.lookup key <;> simp_all
+      have := ntable1LookupImpSlots1 _ _ h
+      simp_all
+
+    have : ∀ (j : ℤ), OfNat.ofNat 0 ≤ j → j < i'.val → slots1.val.index j = AList.Nil := by
+      intro j h0 h1
+      if h : j = i.val then
+        simp_all
+      else
+        have := hEmpty j h0 (by scalar_tac)
+        simp_all
+
+    have : ntable1.al_v.len + (Slots.al_v slots1).len ≤ Usize.max := by
+      have : i.val < (List.map AList.v slots.val).len := by simp; scalar_tac
+      simp_all [Slots.al_v, List.len_flatten_update_eq, List.map_update_eq]
+
+    have : n = slots1.val.len - i'.val := by simp_all; scalar_tac
+
+    progress as ⟨ ntable2, slots2, _, _, hLookup2Rev, hLookup21, hLookup22, hIndexNil ⟩
+
+    simp [and_assoc]
+    have : ∀ (j : ℤ), OfNat.ofNat 0 ≤ j → j < slots2.val.len → slots2.val.index j = AList.Nil := by
+      intro j h0 h1
+      apply hIndexNil j h0 h1
+    have : ntable2.al_v.len = ntable.al_v.len + slots.al_v.len := by simp_all [Slots.al_v]
+    have : ∀ key v, ntable2.lookup key = some v →
+           ntable.lookup key = some v ∨ slots.lookup key = some v := by
+      intro key v hLookup
+      apply move_slots_updated_table_lookup_imp ntable ntable1 ntable2 slots slots1 slot hIneq <;>
+      try assumption
+    have hLookupPreserve :
+      (∀ key v, slots.lookup key = some v → ntable2.lookup key = some v) ∧
+      (∀ key v, ntable.lookup key = some v → ntable2.lookup key = some v) := by
+      exact move_one_slot_lookup_equiv ntable ntable1 ntable2 slot slots slots1 i.val
+        (by assumption) (by assumption) (by assumption)
+        (by assumption) (by assumption) (by assumption) (by assumption)
+    simp_all [alloc.vec.Vec.len, or_assoc]
+    apply hLookupPreserve
+  else
+    simp [hi, and_assoc, *]
+    simp_all
+    have hi : i = alloc.vec.Vec.len (AList α) slots := by scalar_tac
+    have hEmpty : ∀ j, 0 ≤ j → j < slots.val.len → slots.val.index j = AList.Nil := by
+      simp [hi] at hEmpty
+      exact hEmpty
+    have hNil : slots.al_v = [] := slots_forall_nil_imp_al_v_nil slots hEmpty
+    have hLenNonZero : slots.val.len ≠ 0 := by simp [*]
+    have hLookupEmpty := slots_forall_nil_imp_lookup_none slots hLenNonZero hEmpty
+    simp [hNil, hLookupEmpty]
+    apply hEmpty
+
+@[pspec]
+theorem move_elements_spec
+  {α : Type} (ntable : HashMap α) (slots : Slots α)
+  (hinv : ntable.inv)
+  (hslotsNempty : 0 < slots.val.len)
+  (hSlotsInv : slots_t_inv slots)
+  -- The initial table is empty
+  (hEmpty : ∀ key, ntable.lookup key = none)
+  (hTableLen : ntable.al_v.len = 0)
+  (hSlotsLen : slots.al_v.len ≤ Usize.max)
+  :
+  ∃ ntable1 slots1, ntable.move_elements α slots = ok (ntable1, slots1) ∧
+  ntable1.inv ∧
+  ntable1.al_v.len = ntable.al_v.len + slots.al_v.len ∧
+  (∀ key v, ntable1.lookup key = some v ↔ slots.lookup key = some v)
+  := by
+  rw [move_elements]
+  let n := (slots.val.len - 0).toNat
+  have hn : n = slots.val.len - 0 := by
+    -- TODO: scalar_tac should succeed here
+    scalar_tac_preprocess
+    simp [n] at *
+    norm_cast at *
+    have := @Int.le_toNat n (slots.val.len - OfNat.ofNat 0) (by simp; scalar_tac)
+    simp_all
+  have ⟨ ntable1, slots1, hEq, _, _, ntable1Lookup, slotsLookup, _, _ ⟩ :=
+    move_elements_loop_spec (slots.val.len - 0).toNat ntable slots 0#usize hn (by scalar_tac) hinv
+    (by scalar_tac)
+    hSlotsInv
+    (by intro j h0 h1; scalar_tac)
+    (by simp [*])
+    (by simp [*])
+    (by scalar_tac)
+  simp [hEq]; clear hEq
+  split_conjs <;> try assumption
+  intro key v
+  have := ntable1Lookup key v
+  have := slotsLookup key v
+  constructor <;> simp_all
+
+@[pspec]
+theorem try_resize_spec {α : Type} (hm : HashMap α) (hInv : hm.inv):
+  ∃ hm', hm.try_resize α = ok hm' ∧
+  (∀ key, hm'.lookup key = hm.lookup key) ∧
+  hm'.al_v.len = hm.al_v.len := by
+  rw [try_resize]
+  simp
+  progress as ⟨ n1 ⟩ -- TODO: simplify (Usize.ofInt (OfNat.ofNat 2) try_resize.proof_1).val
+  have : hm.2.1.val ≠ 0 := by
+    simp [inv, inv_load] at hInv
+    -- TODO: why does hm.max_load_factor appears as hm.2??
+    -- Can we deactivate field notations?
+    omega
+  progress as ⟨ n2 ⟩
+  if hSmaller : hm.slots.val.len ≤ n2.val then
+    simp [hSmaller]
+    have : (alloc.vec.Vec.len (AList α) hm.slots).val * 2 ≤ Usize.max := by
+          simp [alloc.vec.Vec.len, inv, inv_load] at *
+          -- TODO: this should be automated
+          have hIneq1 : n1.val ≤ Usize.max / 2 := by simp [*]
+          simp [Int.le_ediv_iff_mul_le] at hIneq1
+          -- TODO: this should be automated
+          have hIneq2 : n2.val ≤ n1.val / hm.2.1.val := by simp [*]
+          rw [Int.le_ediv_iff_mul_le] at hIneq2 <;> try simp [*]
+          have : n2.val * 1 ≤ n2.val * hm.max_load_factor.1.val := by
+            apply Int.mul_le_mul <;> scalar_tac
+          scalar_tac
+    progress as ⟨ newLength ⟩
+    have : 0 < newLength.val := by
+      simp_all [inv, inv_load]
+    progress as ⟨ ntable1 .. ⟩ -- TODO: introduce nice notation to take care of preconditions
+    . -- Pre 1
+      simp_all [inv, inv_load]
+      split_conjs at hInv
+      --
+      apply Int.mul_le_of_le_ediv at hSmaller <;> try simp [*]
+      apply Int.mul_le_of_le_ediv at hSmaller <;> try simp
+      --
+      have : (hm.slots.val.len * hm.2.1.val) * 1 ≤ (hm.slots.val.len * hm.2.1.val) * 2 := by
+        apply Int.mul_le_mul <;> (try simp [*]); scalar_tac
+      --
+      ring_nf at *
+      simp [*]
+      unfold max_load max_load_factor at *
+      omega
+    . -- Pre 2
+      simp_all [inv, inv_load]
+      unfold max_load_factor at * -- TODO: this is really annoying
+      omega
+    . -- End of the proof
+      have : slots_t_inv hm.slots := by simp_all [inv] -- TODO
+      have : (Slots.al_v hm.slots).len ≤ Usize.max := by simp_all [inv, al_v, v, Slots.al_v]; scalar_tac
+      progress as ⟨ ntable2, slots1, _, _, hLookup .. ⟩ -- TODO: assumption is not powerful enough
+      simp_all [lookup, al_v, v, alloc.vec.Vec.len]
+      intro key
+      replace hLookup := hLookup key
+      cases h1: (ntable2.slots.val.index (key.val % ntable2.slots.val.len)).v.lookup' key <;>
+      cases h2: (hm.slots.val.index (key.val % hm.slots.val.len)).v.lookup' key <;>
+      simp_all [Slots.lookup]
+  else
+    simp [hSmaller]
+    tauto
+
+@[pspec]
+theorem insert_spec {α} (hm : HashMap α) (key : Usize) (value : α)
+  (hInv : hm.inv)
+  (hNotSat : hm.lookup key = none → hm.len_s < Usize.max) :
+  ∃ hm1, insert α hm key value = ok hm1 ∧
+  --
+  hm1.lookup key = value ∧
+  (∀ key', key' ≠ key → hm1.lookup key' = hm.lookup key') ∧
+  --
+  match hm.lookup key with
+  | none => hm1.len_s = hm.len_s + 1
+  | some _ => hm1.len_s = hm.len_s
+  := by
+  rw [insert]
+  progress as ⟨ hm1 .. ⟩
+  simp [len]
+  split
+  . split
+    . simp [*]
+      intros; tauto
+    . progress as ⟨ hm2 .. ⟩
+      simp [*]
+      intros; tauto
+  . simp [*]; tauto
+
+@[pspec]
+theorem get_in_list_spec {α} (key : Usize) (slot : AList α) (hLookup : slot.lookup key ≠ none) :
+  ∃ v, get_in_list α key slot = ok v ∧ slot.lookup key = some v := by
+  induction slot <;>
+  rw [get_in_list, get_in_list_loop] <;>
+  simp_all [AList.lookup]
+  split <;> simp_all
+
+@[pspec]
+theorem get_spec {α} (hm : HashMap α) (key : Usize) (hInv : hm.inv) (hLookup : hm.lookup key ≠ none) :
+  ∃ v, get α hm key = ok v ∧ hm.lookup key = some v := by
+  rw [get]
+  simp [hash_key, alloc.vec.Vec.len]
+  have : 0 < hm.slots.val.len := by simp_all [inv]
+  progress as ⟨ hash_mod .. ⟩ -- TODO: decompose post by default
+  simp at *
+  have : 0 ≤ hash_mod.val := by -- TODO: automate
+    simp [*]
+    apply Int.emod_nonneg; simp [inv] at hInv; scalar_tac
+  have : hash_mod < hm.slots.val.len := by -- TODO: automate
+    simp [*]
+    apply Int.emod_lt_of_pos; scalar_tac
+  progress as ⟨ slot ⟩
+  progress as ⟨ v .. ⟩ <;> simp_all [lookup]
+
+@[pspec]
+theorem get_mut_in_list_spec {α} (key : Usize) (slot : AList α)
+  {l i : Int}
+  (hInv : slot_t_inv l i slot)
+  (hLookup : slot.lookup key ≠ none) :
+  ∃ v back, get_mut_in_list α slot key = ok (v, back) ∧
+  slot.lookup key = some v ∧
+  ∀ v', ∃ slot', back v' = ok slot' ∧
+    slot_t_inv l i slot' ∧
+    slot'.lookup key = v' ∧
+    (∀ key', key' ≠ key → slot'.lookup key' = slot.lookup key') ∧
+    -- We need this strong post-condition for the recursive case
+    (∀ key', slot.v.allP (fun x => key' ≠ x.1) → slot'.v.allP (fun x => key' ≠ x.1))
+   := by
+  induction slot <;>
+  rw [get_mut_in_list, get_mut_in_list_loop] <;>
+  simp_all [AList.lookup]
+  split
+  . -- Non-recursive case
+    simp_all [and_assoc, slot_t_inv]
+  . -- Recursive case
+    -- TODO: progress doesn't instantiate l correctly
+    rename _ → _ → _ => ih
+    rename AList α => tl
+    replace ih := ih (by simp_all [slot_t_inv]) (by simp_all)
+    -- progress also fails here
+    -- TODO: progress? notation to have some feedback
+    have ⟨ v, back, hEq, _, hBack ⟩ := ih; clear ih
+    simp [hEq]; clear hEq
+    simp [and_assoc, *]
+    -- Proving the post-condition about back
+    intro v
+    progress as ⟨ slot', _, _, _, hForAll ⟩; clear hBack
+    simp [and_assoc, *]
+    constructor
+    . simp_all [slot_t_inv, slot_s_inv, slot_s_inv_hash]
+    . simp_all
+
+@[pspec]
+theorem get_mut_spec {α} (hm : HashMap α) (key : Usize) (hInv : hm.inv) (hLookup : hm.lookup key ≠ none) :
+  ∃ v back, get_mut α hm key = ok (v, back) ∧
+  hm.lookup key = some v ∧
+  ∀ v', ∃ hm', back v' = ok hm' ∧
+    hm'.lookup key = v' ∧
+    ∀ key', key' ≠ key → hm'.lookup key' = hm.lookup key'
+   := by
+  rw [get_mut]
+  simp [hash_key, alloc.vec.Vec.len]
+  have : 0 < hm.slots.val.len := by simp_all [inv]
+  progress as ⟨ hash_mod .. ⟩ -- TODO: decompose post by default
+  simp at *
+  have : 0 ≤ hash_mod.val := by -- TODO: automate
+    simp [*]
+    apply Int.emod_nonneg; simp [inv] at hInv; scalar_tac
+  have : hash_mod < hm.slots.val.len := by -- TODO: automate
+    simp [*]
+    apply Int.emod_lt_of_pos; scalar_tac
+  progress as ⟨ slot, index_back .. ⟩
+  have : slot_t_inv hm.slots.val.len hash_mod slot := by
+    simp_all [inv, slots_t_inv]
+  have : slot.lookup key ≠ none := by
+    simp_all [lookup]
+  progress as ⟨ v, back .. ⟩
+  simp [and_assoc, lookup, *]
+  constructor
+  . simp_all
+  . -- Backward function
+    intro v'
+    progress as ⟨ slot' .. ⟩
+    progress as ⟨ slots' ⟩
+    simp_all
+    -- Last postcondition
+    intro key' hNotEq
+    have : 0 ≤ key'.val % hm.slots.val.len := by -- TODO: automate
+      apply Int.emod_nonneg; simp [inv] at hInv; scalar_tac
+    have : key'.val % hm.slots.val.len < hm.slots.val.len := by -- TODO: automate
+      apply Int.emod_lt_of_pos; scalar_tac
+    -- We need to do a case disjunction
+    cases h: (key.val % hm.slots.val.len == key'.val % hm.slots.val.len) <;>
+    simp_all
+
+@[pspec]
+theorem remove_from_list_spec {α} (key : Usize) (slot : AList α) {l i} (hInv : slot_t_inv l i slot) :
+  ∃ v slot', remove_from_list α key slot = ok (v, slot') ∧
+  slot.lookup key = v ∧
+  slot'.lookup key = none ∧
+  (∀ key', key' ≠ key → slot'.lookup key' = slot.lookup key') ∧
+  match v with
+  | none => slot'.v.len = slot.v.len
+  | some _ => slot'.v.len = slot.v.len - 1 := by
+  rw [remove_from_list, remove_from_list_loop]
+  match hEq : slot with
+  | .Nil =>
+    simp [and_assoc]
+  | .Cons k v0 tl =>
+    simp
+    if hKey : k = key then
+      simp [hKey, and_assoc]
+      simp_all [slot_t_inv, slot_s_inv]
+      apply slot_allP_not_key_lookup
+      simp [*]
+    else
+      simp [hKey]
+      -- TODO: progress doesn't instantiate l properly
+      have hInv' : slot_t_inv l i tl := by simp_all [slot_t_inv]
+      have ⟨ v1, tl1, hRemove, _, _, hLookupTl1, _ ⟩ := remove_from_list_spec key tl hInv'
+      simp [and_assoc, *]; clear hRemove
+      constructor
+      . intro key' hNotEq1
+        simp_all
+      . cases v1 <;> simp_all
+
+theorem lookup'_not_none_imp_len_pos (l : List (Usize × α)) (key : Usize) (hLookup : l.lookup' key ≠ none) :
+  0 < l.len := by
+  induction l <;> simp_all
+  scalar_tac
+
+theorem lookup_not_none_imp_len_s_pos (hm : HashMap α) (key : Usize) (hLookup : hm.lookup key ≠ none)
+  (hNotEmpty : 0 < hm.slots.val.len) :
+  0 < hm.len_s := by
+  have : 0 ≤ key.val % hm.slots.val.len := by -- TODO: automate
+    apply Int.emod_nonneg; scalar_tac
+  have : key.val % hm.slots.val.len < hm.slots.val.len := by -- TODO: automate
+    apply Int.emod_lt_of_pos; scalar_tac
+  have := List.len_index_le_len_flatten hm.v (key.val % hm.slots.val.len)
+  have := lookup'_not_none_imp_len_pos (hm.slots.val.index (key.val % hm.slots.val.len)).v key
+  simp_all [lookup, len_s, al_v, v]
+  scalar_tac
+
+@[pspec]
+theorem remove_spec {α} (hm : HashMap α) (key : Usize) (hInv : hm.inv) :
+  ∃ v hm', remove α hm key = ok (v, hm') ∧
+  hm.lookup key = v ∧
+  hm'.lookup key = none ∧
+  (∀ key', key' ≠ key → hm'.lookup key' = hm.lookup key') ∧
+  match v with
+  | none => hm'.len_s = hm.len_s
+  | some _ => hm'.len_s = hm.len_s - 1 := by
+  rw [remove]
+  simp [hash_key, alloc.vec.Vec.len]
+  have : 0 < hm.slots.val.len := by simp_all [inv]
+  progress as ⟨ hash_mod .. ⟩ -- TODO: decompose post by default
+  simp at *
+  have : 0 ≤ hash_mod.val := by -- TODO: automate
+    simp [*]
+    apply Int.emod_nonneg; simp [inv] at hInv; scalar_tac
+  have : hash_mod < hm.slots.val.len := by -- TODO: automate
+    simp [*]
+    apply Int.emod_lt_of_pos; scalar_tac
+  progress as ⟨ slot, index_back .. ⟩
+  have : slot_t_inv hm.slots.val.len hash_mod slot := by simp_all [inv, slots_t_inv]
+  progress as ⟨ vOpt, slot' .. ⟩
+  match hOpt : vOpt with
+  | none =>
+    simp [*]
+    progress as ⟨ slot'' ⟩
+    simp [and_assoc, lookup, *]
+    simp_all [al_v, v]
+    intro key' hNotEq
+    -- We need to make a case disjunction
+    cases h: (key.val % hm.slots.val.len) == (key'.val % hm.slots.val.len) <;>
+    simp_all
+  | some v =>
+    simp [*]
+    have : 0 < hm.num_entries.val := by
+      have := lookup_not_none_imp_len_s_pos hm key (by simp_all [lookup]) (by simp_all [inv])
+      simp_all [inv]
+    progress as ⟨ newSize .. ⟩
+    progress as ⟨ slots1 .. ⟩
+    simp_all [and_assoc, lookup, al_v, HashMap.v]
+    constructor
+    . intro key' hNotEq
+      cases h: (key.val % hm.slots.val.len) == (key'.val % hm.slots.val.len) <;>
+      simp_all
+    . scalar_tac
 
 end HashMap
 
