backends/lean/Base/Progress/Progress.lean
@@ -131,7 +131,7 @@ def progressWith (fExpr : Expr) (th : TheoremOrLocal)
     Tactic.focus do
     let _ ←
       tryTac
-        (simpAt true {} #[] []
+        (simpAt true {} [] []
                [``Primitives.bind_tc_ok, ``Primitives.bind_tc_fail, ``Primitives.bind_tc_div]
                [hEq.fvarId!] (.targets #[] true))
     -- It may happen that at this point the goal is already solved (though this is rare)
@@ -140,7 +140,7 @@ def progressWith (fExpr : Expr) (th : TheoremOrLocal)
     else
        trace[Progress] "goal after applying the eq and simplifying the binds: {← getMainGoal}"
        -- TODO: remove this (some types get unfolded too much: we "fold" them back)
-       let _ ← tryTac (simpAt true {} #[] [] scalar_eqs [] .wildcard_dep)
+       let _ ← tryTac (simpAt true {} [] [] scalar_eqs [] .wildcard_dep)
        trace[Progress] "goal after folding back scalar types: {← getMainGoal}"
        -- Clear the equality, unless the user requests not to do so
        let mgoal ← do
@@ -410,7 +410,7 @@ namespace Test
     -- This spec theorem is suboptimal, but it is good to check that it works
     progress with Scalar.add_spec as ⟨ z, h1 .. ⟩
     simp [*, h1]
- 
+
   example {x y : U32}
     (hmax : x.val + y.val ≤ U32.max) :
     ∃ z, x + y = ok z ∧ z.val = x.val + y.val := by
